\documentclass[12pt, psamsfonts]{amsart}

%-------Packages---------
\usepackage{amssymb,amsfonts}
\usepackage{semantic}
\usepackage{fullpage}
\usepackage{tikz-cd}
\usepackage{todonotes}
\usepackage{physics}
\usepackage[all,arc]{xy}
\usepackage{enumerate}
\usepackage{enumitem}
\usepackage{mathrsfs}
\usepackage{theoremref}
\usepackage{graphicx}
\usepackage[bookmarks]{hyperref}

%--------Theorem Environments--------
%theoremstyle{plain} --- default
\newtheorem{thm}{Theorem}[section]
\newtheorem{cor}[thm]{Corollary}
\newtheorem{prop}[thm]{Proposition}
\newtheorem{lem}[thm]{Lemma}
\newtheorem{conj}[thm]{Conjecture}
\newtheorem{quest}[thm]{Question}

\theoremstyle{definition}
\newtheorem{defn}[thm]{Definition}
\newtheorem{defns}[thm]{Definitions}
\newtheorem{con}[thm]{Construction}
\newtheorem{exmp}[thm]{Example}
\newtheorem{exmps}[thm]{Examples}
\newtheorem{notn}[thm]{Notation}
\newtheorem{notns}[thm]{Notations}
\newtheorem{addm}[thm]{Addendum}
\newtheorem*{exer}{Exercise}

\theoremstyle{remark}
\newtheorem{rem}[thm]{Remark}
\newtheorem{rems}[thm]{Remarks}
\newtheorem{warn}[thm]{Warning}
\newtheorem{sch}[thm]{Scholium}

\DeclareMathOperator{\Hom}{Hom}
\DeclareMathOperator{\Id}{Id}
\DeclareMathOperator{\End}{End}
\DeclareMathOperator{\ord}{ord}
\DeclareMathOperator{\Aut}{Aut}
\DeclareMathOperator{\Gal}{Gal}

\makeatletter
\let\c@equation\c@thm
\makeatother
\numberwithin{equation}{section}

\bibliographystyle{plain}

\begin{document}

\title{Math 602 (Homework 5)}
\author{Hidenori Shinohara}
\maketitle

\begin{exer}{(1)}
  This can be proved using induction.
  The base case $m = 1$ is trivial.
  Suppose that the proposition has been shown for some $m \in \mathbb{N}$.
  We will show the $(m + 1)$ case.
  By the definition of a determinant,
  \begin{align*}
    \Delta = \sum_{k=1}^{m + 1} (-1)^{k + 1}\det(M_{k, 1})
  \end{align*}
  where $M_{k, 1}$ is the matrix obtained by deleting the $k$th row and 1st column.
  We can apply the inductive hypothesis to each $M_{k, 1}$ because, for instance, when $k = 1$,
  \begin{align*}
    \det(M_{1, 1})
      &= \det\begin{bmatrix}
        \alpha_2 & \alpha_2^2 & \cdots & \alpha_2^m \\
        & \ddots & \\
        \alpha_{m + 1} & \alpha_{m + 1}^2 & \cdots & \alpha_{m + 1}^m
        \end{bmatrix} \\
      &= \alpha_2 \cdots \alpha_{m + 1}\det\begin{bmatrix}
        1 & \alpha_2 & \alpha_2^2 & \cdots & \alpha_2^{m - 1} \\
        & \ddots & \\
        1 & \alpha_{m + 1} & \alpha_{m + 1}^2 & \cdots & \alpha_{m + 1}^{m - 1}
        \end{bmatrix} \\
      &= \alpha_2 \cdots \alpha_{m + 1}\prod_{2 \leq i < j \leq m} (\alpha_j - \alpha_i).
  \end{align*}
  A similar argument can be applied to other cases and we obtain
  \begin{align*}
    \Delta = \sum_{k=1}^{m + 1} (-1)^{k + 1}(\alpha_1 \cdots \hat{\alpha_k} \cdots \alpha_m)\prod_{i < j, i \ne k, j \ne k} (\alpha_j - \alpha_i).
  \end{align*}
  It can be observed that, for each $k = 1, \cdots, m + 1$, the $k$th term $(\alpha_1 \cdots \hat{\alpha_k} \cdots \alpha_m)\prod_{i < j, i \ne k, j \ne k} (\alpha_j - \alpha_i)$ does not contain any $\alpha_k$.
  On the other hand, for any $l \ne k$, every term that we obtain when expanding the $l$th term contains $\alpha_k$.
  Therefore, it suffices to show that, for each $k$, the sum of all the terms in $\prod_{1 \leq i < j \leq m + 1}(\alpha_j - \alpha_i)$ that do not contain $\alpha_k$ is equal to the $k$th term in the above expression.
  \begin{align*}
    \prod_{1 \leq i < j \leq m + 1} (\alpha_j - \alpha_i)
      &= \prod_{k + 1 \leq j} (\alpha_j - \alpha_k)\prod_{j \leq k - 1} (\alpha_k - \alpha_j)\prod_{1 \leq i < j \leq m + 1, i \ne k, j \ne k}(\alpha_j - \alpha_i) \\
      &= (-1)^{k - 1}\prod_{j \ne k} (\alpha_j - \alpha_k)\prod_{1 \leq i < j \leq m + 1, i \ne k, j \ne k}(\alpha_j - \alpha_i) \\
      &= (-1)^{k - 1}(\alpha_1 \cdots \hat{\alpha_k} \cdots \alpha_{m + 1})\prod_{1 \leq i < j \leq m + 1, i \ne k, j \ne k}(\alpha_j - \alpha_i) + \alpha_kF(\alpha_1, \cdots, \alpha_{m + 1}) \\
      &= (-1)^{k + 1}(\alpha_1 \cdots \hat{\alpha_k} \cdots \alpha_{m + 1})\prod_{1 \leq i < j \leq m + 1, i \ne k, j \ne k}(\alpha_j - \alpha_i) + \alpha_kF(\alpha_1, \cdots, \alpha_{m + 1})
  \end{align*}
  for some polynomial $F$.

  $\Delta^2 \ne \prod_{i \ne j}(\alpha_j - \alpha_i)$ in general.
  Let $\alpha_1 = 0, \alpha_2 = 1$.
  Then $\det(A)^2 = \det\begin{bmatrix} 1 & 0 \\ 1 & 1 \end{bmatrix}^2 = 1$.
  On the other hand, $\prod_{i \ne j}(\alpha_j - \alpha_i) = (0 - 1)(1 - 0) = -1$.
\end{exer}

\begin{exer}{(6)}
  Let $ab \in \sqrt{q}$.
  Then $a^nb^n \in q$ for some $n \in \mathbb{N}$.
  Then $a^n \in q$ or $(b^n)^m \in q$ for some $m \in \mathbb{N}$.
  If $a^n \in q$, then $a \in \sqrt{q}$.
  If $b^{nm} \in q$, then $b \in \sqrt{q}$.
  Therefore, $\sqrt{q}$ is prime.

  Let $f:A \rightarrow B$ be given and $q$ be a primary ideal of $B$.
  Let $ab \in f^{-1}(q)$.
  Then $f(a)f(b) \in q$, so $f(a) \in q$ or $(f(b))^m \in q$ for some $m \geq 1$.
  If $f(a) \in q$, then $a \in f^{-1}(q)$.
  If $f(b^m) \in q$, then $b^m \in f^{-1}(q)$.
  Therefore, $f^{-1}(q)$ is primary.
\end{exer}

\end{document}


