\documentclass[12pt, psamsfonts]{amsart}

%-------Packages---------
\usepackage{amssymb,amsfonts}
\usepackage{fullpage}
\usepackage{tikz-cd}
\usepackage{todonotes}
\usepackage{physics}
\usepackage[all,arc]{xy}
\usepackage{enumerate}
\usepackage{enumitem}
\usepackage{mathrsfs}
\usepackage{theoremref}
\usepackage{graphicx}
\usepackage[bookmarks]{hyperref}

%--------Theorem Environments--------
%theoremstyle{plain} --- default
\newtheorem{thm}{Theorem}[section]
\newtheorem{cor}[thm]{Corollary}
\newtheorem{prop}[thm]{Proposition}
\newtheorem{lem}[thm]{Lemma}
\newtheorem{conj}[thm]{Conjecture}
\newtheorem{quest}[thm]{Question}

\theoremstyle{definition}
\newtheorem{defn}[thm]{Definition}
\newtheorem{defns}[thm]{Definitions}
\newtheorem{con}[thm]{Construction}
\newtheorem{exmp}[thm]{Example}
\newtheorem{exmps}[thm]{Examples}
\newtheorem{notn}[thm]{Notation}
\newtheorem{notns}[thm]{Notations}
\newtheorem{addm}[thm]{Addendum}
\newtheorem*{exer}{Exercise}

\theoremstyle{remark}
\newtheorem{rem}[thm]{Remark}
\newtheorem{rems}[thm]{Remarks}
\newtheorem{warn}[thm]{Warning}
\newtheorem{sch}[thm]{Scholium}

\DeclareMathOperator{\Hom}{Hom}
\DeclareMathOperator{\Id}{Id}
\DeclareMathOperator{\End}{End}
\DeclareMathOperator{\ord}{ord}
\DeclareMathOperator{\Aut}{Aut}

\makeatletter
\let\c@equation\c@thm
\makeatother
\numberwithin{equation}{section}

\bibliographystyle{plain}

\begin{document}

\title{Math 611 (Due 11/13)}
\author{Hidenori Shinohara}
\maketitle

\section{Simplicial and Singular Homology}

\begin{exer}{(Problem 27)}
  Let $f:(X, A) \rightarrow (Y, B)$ be a map such that both $f: X \rightarrow Y, f:A \rightarrow B$ are homotopy equivalences.

  \begin{itemize}
    \item
      Show that $f_* : H_n(X, A) \rightarrow  H_n(Y, B)$ is an isomorphism for all $n$.
    \item
      For the case of the inclusion $f:(D^n, S^{n - 1}) \rightarrow (D^n, D^n \setminus \{ 0 \})$, show that $f$ is not a homotopy equivalence of pairs -
      there is no $g: (D^n, D^n \setminus \{ 0 \}) \rightarrow (D^n, S^{n - 1})$ such that $fg$ and $gf$ are homotopic to the identity through maps of pairs.
  \end{itemize}
\end{exer}

\begin{proof}
  $ $
  \begin{itemize}
    \item
      For each $n \geq 1$, we have an exact sequence $H_n(A) \rightarrow H_n(X) \rightarrow H_n(X, A) \rightarrow H_{n - 1}(A) \rightarrow H_{n - 1}(X)$ and another one with $X, A$ replaced with $Y, B$.
      Moreover, they are connected by homomorphisms $f_*: H_n(A) \rightarrow H_n(B), f_*: H_n(X) \rightarrow H_n(Y), f_*:H_n(X, A) \rightarrow H_n(Y, B)$ such that the diagram commutes. (naturality)
      Since $f: X \rightarrow Y$ and $f: A \rightarrow B$ are both homotopy equivalences, $f_*: H_n(X) \rightarrow H_n(Y), f_*: H_n(A) \rightarrow H_n(B)$ are isomorphisms.
      By the Five lemma, $f_*: H_n(X, A) \rightarrow H_n(X, B)$ is an isomorphism.

      The exact sequence $H_1(A) \rightarrow H_1(X) \rightarrow H_1(X, A) \rightarrow 0$ can be extended to $H_1(A) \rightarrow H_1(X) \rightarrow H_1(X, A) \rightarrow 0 \rightarrow 0$ by appending 0 at the end.
      Using the same argument as above, $f_*: H_1(X, A) \rightarrow H_1(Y, B)$ is an isomorphism.
    \item
      Suppose $f: (D^n, S^{n - 1}) \rightarrow (D^n, D^n - \{ 0 \})$ is a homotopy equivalence.
      Then there exists a $g: (D^n, D^n - \{ 0 \}) \rightarrow (D^n, S^{n - 1})$ such that $f \circ g$ and $g \circ f$ are homotopic to the identity maps in corresponding domains.
      Since $g$ is continuous, $g(\overline{D^n - \{ 0 \}}) = \overline{g(D^n - \{ 0 \})} \subset \overline{S^{n - 1}} = S^{n - 1}$.
      Therefore, $g$ maps $D^n$ into $S^{n - 1}$.
      Since $f$ maps $S^{n - 1}$ into $D^n$, $g \circ f$ maps $S^{n - 1}$ into $S^{n - 1}$.
      We know this is homotopic to the identity map from the problem statement.
      Similarly, $f \circ g$ maps $D^n$ into $D^n$ and we know this is homotopic to the identity map from the problem statement.
      Therefore, this implies that $D^n$ and $S^{n - 1}$ are homotopy equivalent.
      However, this is false because $D^n$ is contractible but $S^{n - 1}$ is not.

      Hence, $f$ cannot be homotopy equivalent.
  \end{itemize}

\end{proof}

\end{document}


